monadic cleanup

monadic.dfy
@@ -12,59 +12,75 @@ datatype Term  =
   | Or(e : Term, e' : Term)
   | EqZ(e : Term)
   | Record(em : seq<(string,Term)>)
+  | RecordProj(e : Term, f : string)
 
 datatype Val = IntVal(v : int) | BoolVal(b : bool) | RecordVal(m : map<string,Val>)
 
 type Env = map<string,Val>
 
-function eval(env : Env, e : Term) : Option<Val> {
+function eval(env : Env, e : Term) : Option<Val>
+    decreases e , 0
+{
   match e {
-    case Var(x) => if x in env then Some(env[x]) else None
+    case Var(x) => lookup(env,x)
     case Add(e,e') => 
-        var v1 :- eval(env,e);
-        var v2 :- eval(env,e');
-        valAdd(v1,v2)
+        var n1 :- evalInt(env,e);
+        var n2 :- evalInt(env,e');
+        Some(IntVal(n1 + n2))
     case Or(e,e') =>
-        var v1 :- eval(env,e);
-        var v2 :- eval(env,e');
-        valOr(v1,v2)
+        var b1 :- evalBool(env,e);
+        var b2 :- evalBool(env,e');
+        Some(BoolVal(b1 || b2))
     case EqZ(e) => 
-        var v :- eval(env,e);
-        valEqZ(v)
-    case Record(em) => match evalRecord(env,em) {
-      case Some(m) => Some(RecordVal(m))
-      case _ => None
-    }
+        var n :- evalInt(env,e);
+        Some(BoolVal(n == 0))
+    case Record(em) =>
+        var m :- evalRecordExpr(env,em);
+        Some(RecordVal(m))
+    case RecordProj(e,f) => 
+        var m :- evalRecord(env,e);
+        lookup(m,f)
   }
 }
 
-function valAdd(v1 : Val, v2 : Val) : Option<Val> {
-    match (v1,v2) {
-        case (IntVal(n), IntVal(m)) => Some (IntVal (n + m))
-        case _ => None
-    }
-}
-
-function valOr(v1 : Val, v2 : Val) : Option<Val> {
-    match (v1,v2) {
-        case (BoolVal(n), BoolVal(m)) => Some (BoolVal (n || m))
-        case _ => None
-    }
-}
-
-function valEqZ(v : Val) : Option<Val> {
+function evalInt(env : Env, e : Term) : Option<int>
+    decreases e , 1
+{
+    var v :- eval(env,e);
     match v {
-        case IntVal(n) => if n == 0 then Some(BoolVal(true)) else Some(BoolVal(false))
+        case IntVal(n) => Some(n)
         case _ => None
     }
 }
 
-function evalRecord(env : Env, es : seq<(string,Term)>) : Option<map<string,Val>> {
+function evalBool(env : Env, e : Term) : Option<bool>
+    decreases e , 1
+{
+    var v :- eval(env,e);
+    match v {
+        case BoolVal(b) => Some(b)
+        case _ => None
+    }
+}
+
+function evalRecord(env : Env, e : Term) : Option<map<string,Val>>
+    decreases e , 1
+{
+    var v :- eval(env,e);
+    match v {
+        case RecordVal(m) => Some(m)
+        case _ => None
+    }
+}
+
+function evalRecordExpr(env : Env, es : seq<(string,Term)>) : Option<map<string,Val>>
+    decreases es
+{
   if es == [] then Some(map[])
   else
     var k := es[0].0;
     var v :- eval(env,es[0].1);
-    var vm :- evalRecord(env,es[1..]);
+    var vm :- evalRecordExpr(env,es[1..]);
     if k in vm.Keys then Some(vm) else Some(vm[k := v])
 }
 
@@ -72,42 +88,74 @@ datatype Ty = IntTy | BoolTy | RecordTy(rm : map<string,Ty>)
 
 type Ctx = map<string,Ty>
 
-function infer(ctx : Ctx, e : Term) : Option<Ty> {
+function infer(ctx : Ctx, e : Term) : Option<Ty>
+    decreases e, 0
+{
   match e {
     case Var(x) => if x in ctx then Some(ctx[x]) else None
     case Add(e,e') => 
-        var t1 :- infer(ctx,e);
-        var t2 :- infer(ctx,e');
-        var _ :- guard(t1 == IntTy);
-        var _ :- guard(t2 == IntTy);
+        var _ :- inferIntTy(ctx,e);
+        var _ :- inferIntTy(ctx,e');
         Some(IntTy)
 
     case Or(e,e') =>
-        var t1 :- infer(ctx,e);
-        var t2 :- infer(ctx,e');
-        var _ :- guard(t1 == BoolTy);
-        var _ :- guard(t2 == BoolTy);
+        var _ :- inferBoolTy(ctx,e);
+        var _ :- inferBoolTy(ctx,e');
         Some(BoolTy)
 
     case EqZ(e) => 
-        var t :- infer(ctx,e);
-        var _ :- guard(t == IntTy);
+        var _ :- inferIntTy(ctx,e);
         Some(BoolTy)
 
     case Record(es) =>
-        var tm :- inferRecord(ctx,es);
+        var tm :- inferRecordExpr(ctx,es);
         Some(RecordTy(tm))
+    
+    case RecordProj(e,f) =>
+        var m :- inferRecordTy(ctx,e);
+        lookup(m,f)
   }
 }
 
-function inferRecord(ctx : Ctx, es : seq<(string,Term)>) : Option<map<string,Ty>> {
+function inferIntTy(ctx : Ctx, e : Term) : Option<()>
+    decreases e, 1
+{
+    var t :- infer(ctx,e);
+    match t {
+        case IntTy => Some(())
+        case _ => None
+    }
+}
+
+function inferBoolTy(ctx : Ctx, e : Term) : Option<()>
+    decreases e, 1
+{
+    var t :- infer(ctx,e);
+    match t {
+        case BoolTy => Some(())
+        case _ => None
+    }
+}
+
+function inferRecordTy(ctx : Ctx, e : Term) : Option<map<string,Ty>>
+    decreases e, 1
+{
+    var t :- infer(ctx,e);
+    match t {
+        case RecordTy(m) => Some(m)
+        case _ => None
+    }
+}
+
+function inferRecordExpr(ctx : Ctx, es : seq<(string,Term)>) : Option<map<string,Ty>>
+    decreases es
+{
   if es == [] then Some(map[])
   else
     var k := es[0].0;
-    match (infer(ctx,es[0].1), inferRecord(ctx,es[1..])) {
-      case (Some(t),Some(tm)) => if k in tm then Some(tm) else Some(tm[k := t])
-      case _ => None
-    }
+    var t :- infer(ctx,es[0].1);
+    var tm :- inferRecordExpr(ctx,es[1..]);
+    if k in tm then Some(tm) else Some(tm[k := t])
 }
 
 function valHasType(v : Val, t : Ty) : bool {
@@ -130,7 +178,7 @@ lemma sound (env : Env, ctx : Ctx, e : Term)
     case Or(e,e') => sound(env,ctx,e); sound(env,ctx,e');
     case EqZ(e) => sound(env,ctx,e);
     case Record(es) =>
-      var mt :| inferRecord(ctx,es) == Some(mt);
+      var mt :| inferRecordExpr(ctx,es) == Some(mt);
       invertRecordTck(ctx,es);
       forall i | 0 <= i < |es|
         ensures eval(env,es[i].1).Some? && valHasType(eval(env,es[i].1).value,infer(ctx,es[i].1).value)
@@ -138,22 +186,23 @@ lemma sound (env : Env, ctx : Ctx, e : Term)
         sound(env,ctx,es[i].1);
       }
       recordEvalLemma(env,es);
+    case RecordProj(e,f) => sound(env,ctx,e);
   }
 }
 
 lemma invertRecordTck(ctx : Ctx, es : seq<(string,Term)>)
-  requires inferRecord(ctx,es).Some?
+  requires inferRecordExpr(ctx,es).Some?
   ensures forall i | 0 <= i < |es| :: infer(ctx,es[i].1).Some?
   // Every result term in es typechecks, and every key appears in the result.
-  ensures forall i | 0 <= i < |es| :: es[i].0 in inferRecord(ctx,es).value.Keys
+  ensures forall i | 0 <= i < |es| :: es[i].0 in inferRecordExpr(ctx,es).value.Keys
   //For every key in the output, it existed in the input, and its type is the result of inferring the type of the last instance of k.
-  ensures forall k | k in inferRecord(ctx,es).value.Keys :: KeyExists(k,es) && infer(ctx,LastOfKey(k,es)).value == inferRecord(ctx,es).value[k]
+  ensures forall k | k in inferRecordExpr(ctx,es).value.Keys :: KeyExists(k,es) && infer(ctx,LastOfKey(k,es)).value == inferRecordExpr(ctx,es).value[k]
 {}
 
 lemma recordEvalLemma(env : Env, es : seq<(string,Term)>)
   requires forall i | 0 <= i < |es| :: eval(env,es[i].1).Some?
-  ensures evalRecord(env,es).Some?
-  ensures forall i | 0 <= i < |es| :: es[i].0 in evalRecord(env,es).value.Keys
-  ensures forall k | k in evalRecord(env,es).value.Keys :: KeyExists(k,es) && eval(env,LastOfKey(k,es)).value == evalRecord(env,es).value[k]
+  ensures evalRecordExpr(env,es).Some?
+  ensures forall i | 0 <= i < |es| :: es[i].0 in evalRecordExpr(env,es).value.Keys
+  ensures forall k | k in evalRecordExpr(env,es).value.Keys :: KeyExists(k,es) && eval(env,LastOfKey(k,es)).value == evalRecordExpr(env,es).value[k]
 {
 }
